

random\_tariff\_2025\_mm\_dd.dfw: Random Tariff Wars

#1: CaseMode := Sensitive

#2: InputMode := Word

eq (1): Demand system

#3:  $pxh = \alpha - \beta \cdot xh - \gamma \cdot yh$

#4:  $pyh = \alpha - \gamma \cdot xh - \beta \cdot yh$

#5:  $pxf = \alpha - \beta \cdot xf - \gamma \cdot yf$

#6:  $pyf = \alpha - \gamma \cdot xf - \beta \cdot yf$

Let  $\lambda$  be prob  $t=T \Rightarrow 1-\lambda$  prob  $t=0$

eq (2): expected profit of x

#7:  $e\text{profit}xh = (pxh - c) \cdot xh$

#8:  $e\text{profit}xf = \lambda \cdot (pxf - c - T) \cdot xf + (1 - \lambda) \cdot (pxf - c) \cdot xf$

#9:  $e\text{profit}x = (pxh - c) \cdot xh + \lambda \cdot (pxf - c - T) \cdot xf + (1 - \lambda) \cdot (pxf - c) \cdot xf$

eq (3): expected profit of y

#10:  $e\text{profit}yf = (pyf - c) \cdot yf$

#11:  $e\text{profit}yh = \lambda \cdot (pyh - c - T) \cdot yh + (1 - \lambda) \cdot (pyh - c) \cdot yh$

#12:  $e\text{profit}y = (pyf - c) \cdot yf + \lambda \cdot (pyh - c - T) \cdot yh + (1 - \lambda) \cdot (pyh - c) \cdot yh$

Derivation of (4) and Appendix A

#13:  $e\text{profit}x = ((\alpha - \beta \cdot xh - \gamma \cdot yh) - c) \cdot xh + \lambda \cdot ((\alpha - \beta \cdot xf - \gamma \cdot yf) - c - T) \cdot xf + (1 - \lambda) \cdot ((\alpha - \beta \cdot xf -$

$$\gamma \cdot yf) - c) \cdot xf$$

$$\#14: \frac{d}{d \, xf} (\text{eprofit}_x = ((\alpha - \beta \cdot xh - \gamma \cdot yh) - c) \cdot xh + \lambda \cdot ((\alpha - \beta \cdot xf - \gamma \cdot yf) - c - T) \cdot xf + (1 - \lambda) \cdot ((\alpha -$$

$$\beta \cdot xf - \gamma \cdot yf) - c) \cdot xf)$$

$$\#15: \quad \quad \quad 0 = -T \cdot \lambda - c - 2 \cdot xf \cdot \beta - yf \cdot \gamma + \alpha$$

$$\#16: \frac{d}{d \, xh} (\text{eprofit}_x = ((\alpha - \beta \cdot xh - \gamma \cdot yh) - c) \cdot xh + \lambda \cdot ((\alpha - \beta \cdot xf - \gamma \cdot yf) - c - T) \cdot xf + (1 - \lambda) \cdot ((\alpha -$$

$$\beta \cdot xf - \gamma \cdot yf) - c) \cdot xf)$$

$$\#17: \quad \quad \quad 0 = -c - 2 \cdot xh \cdot \beta - yh \cdot \gamma + \alpha$$

$$\#18: \text{eprofit}_y = ((\alpha - \gamma \cdot xf - \beta \cdot yf) - c) \cdot yf + \lambda \cdot ((\alpha - \gamma \cdot xh - \beta \cdot yh) - c - T) \cdot yh + (1 - \lambda) \cdot ((\alpha - \gamma \cdot xh - \beta \cdot yh) - c) \cdot yh$$

$$\#19: \frac{d}{d \, yf} (\text{eprofit}_y = ((\alpha - \gamma \cdot xf - \beta \cdot yf) - c) \cdot yf + \lambda \cdot ((\alpha - \gamma \cdot xh - \beta \cdot yh) - c - T) \cdot yh + (1 - \lambda) \cdot ((\alpha -$$

$$\gamma \cdot xh - \beta \cdot yh) - c) \cdot yh)$$

$$\#20: \quad \quad \quad 0 = -c - xf \cdot \gamma - 2 \cdot yf \cdot \beta + \alpha$$

$$\#21: \frac{d}{d \, yh} (\text{eprofit}_y = ((\alpha - \gamma \cdot xf - \beta \cdot yf) - c) \cdot yf + \lambda \cdot ((\alpha - \gamma \cdot xh - \beta \cdot yh) - c - T) \cdot yh + (1 - \lambda) \cdot ((\alpha -$$

$$\gamma \cdot x_h - \beta \cdot y_h) - c) \cdot y_h)$$

$$\#22: \quad 0 = -T \cdot \lambda - c - x_h \cdot \gamma - 2 \cdot y_h \cdot \beta + \alpha$$

$$\#23: \quad \text{SOLVE}([0 = -T \cdot \lambda - c - 2 \cdot x_f \cdot \beta - y_f \cdot \gamma + \alpha, 0 = -c - 2 \cdot x_h \cdot \beta - y_h \cdot \gamma + \alpha, 0 = -c - x_f \cdot \gamma - 2 \cdot y_f \cdot \beta + \alpha, \\ 0 = -T \cdot \lambda - c - x_h \cdot \gamma - 2 \cdot y_h \cdot \beta + \alpha], [x_f, x_h, y_f, y_h])$$

eq (4) sales levels

$$\#24: \quad \left[ x_f = \frac{2 \cdot T \cdot \beta \cdot \lambda + (c - \alpha) \cdot (2 \cdot \beta - \gamma)}{\gamma^2 - 4 \cdot \beta^2} \wedge x_h = \frac{T \cdot \gamma \cdot \lambda + (c - \alpha) \cdot (\gamma - 2 \cdot \beta)}{4 \cdot \beta^2 - \gamma^2} \wedge y_f = \frac{T \cdot \gamma \cdot \lambda + (c - \alpha) \cdot (\gamma - 2 \cdot \beta)}{4 \cdot \beta^2 - \gamma^2} \wedge y_h = \frac{2 \cdot T \cdot \beta \cdot \lambda + (c - \alpha) \cdot (2 \cdot \beta - \gamma)}{\gamma^2 - 4 \cdot \beta^2} \right]$$

$x_f = y_h > 0$  if

$$\#25: \quad 2 \cdot T \cdot \beta \cdot \lambda + (c - \alpha) \cdot (2 \cdot \beta - \gamma) < 0$$

$$\#26: \quad \text{SOLVE}(2 \cdot T \cdot \beta \cdot \lambda + (c - \alpha) \cdot (2 \cdot \beta - \gamma) < 0, T)$$

$$\#27: \quad \text{IF} \left( \beta \cdot \lambda < 0, T > \frac{(c - \alpha) \cdot (\gamma - 2 \cdot \beta)}{2 \cdot \beta \cdot \lambda} \right) \vee \text{IF} \left( \beta \cdot \lambda > 0, T < \frac{(c - \alpha) \cdot (\gamma - 2 \cdot \beta)}{2 \cdot \beta \cdot \lambda} \right)$$

Assumption 3

$$\#28: \quad T < \frac{(c - \alpha) \cdot (\gamma - 2 \cdot \beta)}{2 \cdot \beta \cdot \lambda}$$

soc in Appendix A

$$\#29: \frac{d}{d x_f} \frac{d}{d x_f} (\text{eprofit}_x = ((\alpha - \beta \cdot x_h - \gamma \cdot y_h) - c) \cdot x_h + \lambda \cdot ((\alpha - \beta \cdot x_f - \gamma \cdot y_f) - c - T) \cdot x_f + (1 - \lambda) \cdot ((\alpha - \beta \cdot x_f - \gamma \cdot y_f) - c) \cdot x_f)$$

$$\#30: 0 > -2 \cdot \beta$$

$$\#31: \frac{d}{d x_h} \frac{d}{d x_h} (\text{eprofit}_x = ((\alpha - \beta \cdot x_h - \gamma \cdot y_h) - c) \cdot x_h + \lambda \cdot ((\alpha - \beta \cdot x_f - \gamma \cdot y_f) - c - T) \cdot x_f + (1 - \lambda) \cdot ((\alpha - \beta \cdot x_f - \gamma \cdot y_f) - c) \cdot x_f)$$

$$\#32: 0 > -2 \cdot \beta$$

$$\#33: \frac{d}{d x_h} \frac{d}{d x_f} (\text{eprofit}_x = ((\alpha - \beta \cdot x_h - \gamma \cdot y_h) - c) \cdot x_h + \lambda \cdot ((\alpha - \beta \cdot x_f - \gamma \cdot y_f) - c - T) \cdot x_f + (1 - \lambda) \cdot ((\alpha - \beta \cdot x_f - \gamma \cdot y_f) - c) \cdot x_f)$$

$$\#34: 0 = 0$$

$$\#35: \frac{d}{d y_f} \frac{d}{d y_f} (\text{eprofit}_y = ((\alpha - \gamma \cdot x_f - \beta \cdot y_f) - c) \cdot y_f + \lambda \cdot ((\alpha - \gamma \cdot x_h - \beta \cdot y_h) - c - T) \cdot y_h + (1 - \lambda) \cdot ((\alpha - \gamma \cdot x_h - \beta \cdot y_h) - c) \cdot y_h)$$

$$\#36: 0 > -2 \cdot \beta$$

$$\#37: \frac{d}{d y_h} \frac{d}{d y_h} (\text{eprofit} = ((\alpha - \gamma \cdot x_f - \beta \cdot y_f) - c) \cdot y_f + \lambda \cdot ((\alpha - \gamma \cdot x_h - \beta \cdot y_h) - c - T) \cdot y_h + (1 - \lambda) \cdot ((\alpha - \gamma \cdot x_h - \beta \cdot y_h) - c) \cdot y_h)$$

$$\#38: 0 > -2 \cdot \beta$$

$$\#39: \frac{d}{d y_f} \frac{d}{d y_h} (\text{eprofit} = ((\alpha - \gamma \cdot x_f - \beta \cdot y_f) - c) \cdot y_f + \lambda \cdot ((\alpha - \gamma \cdot x_h - \beta \cdot y_h) - c - T) \cdot y_h + (1 - \lambda) \cdot ((\alpha - \gamma \cdot x_h - \beta \cdot y_h) - c) \cdot y_h)$$

$$\#40: 0 = 0$$

eq (5): equilibrium prices

$$\#41: p_{xh} = \frac{T \cdot \beta \cdot \gamma \cdot \lambda + (2 \cdot \beta - \gamma) \cdot (c \cdot (\beta + \gamma) + \alpha \cdot \beta)}{4 \cdot \beta^2 - \gamma^2}$$

$$\#42: p_{yh} = \frac{T \cdot \lambda \cdot (2 \cdot \beta^2 - \gamma^2) + (2 \cdot \beta - \gamma) \cdot (c \cdot (\beta + \gamma) + \alpha \cdot \beta)}{4 \cdot \beta^2 - \gamma^2}$$

$$\#43: p_{xf} = \frac{T \cdot \lambda \cdot (2 \cdot \beta^2 - \gamma^2) + (2 \cdot \beta - \gamma) \cdot (c \cdot (\beta + \gamma) + \alpha \cdot \beta)}{4 \cdot \beta^2 - \gamma^2}$$

#44:

$$pyf = \frac{T \cdot \beta \cdot \gamma \cdot \lambda + (2 \cdot \beta - \gamma) \cdot (c \cdot (\beta + \gamma) + \alpha \cdot \beta)}{4 \cdot \beta^2 - \gamma^2}$$

eq (7) profits in domestic markets

#45:

$$eprofitxh = \frac{\beta \cdot (T \cdot \gamma \cdot \lambda + (c - \alpha) \cdot (\gamma - 2 \cdot \beta))^2}{(4 \cdot \beta^2 - \gamma^2)^2}$$

#46:

$$eprofityf = \frac{\beta \cdot (T \cdot \gamma \cdot \lambda + (c - \alpha) \cdot (\gamma - 2 \cdot \beta))^2}{(4 \cdot \beta^2 - \gamma^2)^2}$$

eq (8) profits in export markets

#47:

$$eprofitxf = \frac{\beta \cdot (2 \cdot T \cdot \beta \cdot \lambda + (c - \alpha) \cdot (2 \cdot \beta - \gamma))^2}{(4 \cdot \beta^2 - \gamma^2)^2}$$

#48:

$$eprofityh = \frac{\beta \cdot (2 \cdot T \cdot \beta \cdot \lambda + (c - \alpha) \cdot (2 \cdot \beta - \gamma))^2}{(4 \cdot \beta^2 - \gamma^2)^2}$$

Result 2, Appendix B

The condition of this result

$$\#49: T > \frac{(\alpha - c) \cdot (2\beta - \gamma)^2}{4\beta^2 - \gamma^2}$$

Is this consistent with Assumption 3?

$$\#50: \frac{(c - \alpha) \cdot (\gamma - 2\beta)}{2\beta \cdot \lambda} - \frac{(\alpha - c) \cdot (2\beta - \gamma)^2}{4\beta^2 - \gamma^2}$$

eq (B.3)

$$\#51: \frac{(c - \alpha) \cdot (2\beta - \gamma) \cdot (2\beta \cdot (\lambda - 1) - \gamma)}{2\beta \cdot \lambda \cdot (2\beta + \gamma)}$$

> 0 if [always!]

$$\#52: (c - \alpha) \cdot (2\beta - \gamma) \cdot (2\beta \cdot (\lambda - 1) - \gamma) > 0$$

$$\#53: \text{SOLVE}((c - \alpha) \cdot (2\beta - \gamma) \cdot (2\beta \cdot (\lambda - 1) - \gamma) > 0, \lambda)$$

$$\#54: \text{IF}\left(\beta \cdot (c - \alpha) \cdot (2\beta - \gamma) < 0, \lambda < \frac{2\beta + \gamma}{2\beta}\right) \vee \text{IF}\left(\beta \cdot (c - \alpha) \cdot (2\beta - \gamma) > 0, \lambda > \frac{2\beta + \gamma}{2\beta}\right)$$

$$\#55: \lambda < \frac{2\beta + \gamma}{2\beta}$$

$$\#56: \text{eprofitx} = \frac{\beta \cdot (T \cdot \gamma \cdot \lambda + (c - \alpha) \cdot (\gamma - 2\beta))^2}{(4\beta^2 - \gamma^2)^2} + \frac{\beta \cdot (2 \cdot T \cdot \beta \cdot \lambda + (c - \alpha) \cdot (2\beta - \gamma))^2}{(4\beta^2 - \gamma^2)^2}$$

$$\#57: \quad eprofitx = \frac{\beta \cdot (T \cdot \lambda^2 \cdot (4\beta^2 + \gamma^2) + 2 \cdot T \cdot \lambda \cdot (c - \alpha) \cdot (2\beta - \gamma)^2 + 2 \cdot (c - \alpha)^2 \cdot (2\beta - \gamma)^2)}{(4\beta^2 - \gamma^2)^2}$$

$$\#58: \quad \frac{d}{d\lambda} \left( eprofitx = \frac{\beta \cdot (T \cdot \lambda^2 \cdot (4\beta^2 + \gamma^2) + 2 \cdot T \cdot \lambda \cdot (c - \alpha) \cdot (2\beta - \gamma)^2 + 2 \cdot (c - \alpha)^2 \cdot (2\beta - \gamma)^2)}{(4\beta^2 - \gamma^2)^2} \right)$$

eq (B.1) FOC for a minimum

$$\#59: \quad 0 = \frac{2 \cdot T \cdot \beta \cdot (T \cdot \lambda \cdot (4\beta^2 + \gamma^2) + (c - \alpha) \cdot (2\beta - \gamma)^2)}{(4\beta^2 - \gamma^2)^2}$$

$$\#60: \quad \frac{d}{d\lambda} \frac{d}{d\lambda} \left( eprofitx = \frac{\beta \cdot (T \cdot \lambda^2 \cdot (4\beta^2 + \gamma^2) + 2 \cdot T \cdot \lambda \cdot (c - \alpha) \cdot (2\beta - \gamma)^2 + 2 \cdot (c - \alpha)^2 \cdot (2\beta - \gamma)^2)}{(4\beta^2 - \gamma^2)^2} \right)$$

eq (B.2) SOC for minimum

$$\#61: \quad 0 < \frac{2 \cdot T \cdot \beta \cdot (4\beta^2 + \gamma^2)}{(4\beta^2 - \gamma^2)^2}$$

$$\#62: \quad \text{SOLVE} \left( 0 = \frac{2 \cdot T \cdot \beta \cdot (T \cdot \lambda \cdot (4\beta^2 + \gamma^2) + (c - \alpha) \cdot (2\beta - \gamma)^2)}{(4\beta^2 - \gamma^2)^2}, \lambda \right)$$



eq (9)

$$\#63: \quad \lambda_{\text{hat}} = \frac{(\alpha - c) \cdot (2\beta - \gamma)^2}{T \cdot (4\beta^2 + \gamma^2)} \quad \vee \quad T = 0 \quad \vee \quad \beta = 0$$

Result 3 and Appendix C:

$$\#64: \quad \frac{d}{d\lambda} \left( \text{eprofitxh} = \frac{\beta \cdot (T \cdot \gamma \cdot \lambda + (c - \alpha) \cdot (\gamma - 2\beta))^2}{(4\beta^2 - \gamma^2)^2} \right)$$

$$\#65: \quad 0 < \frac{2 \cdot T \cdot \beta \cdot \gamma \cdot (T \cdot \gamma \cdot \lambda + (c - \alpha) \cdot (\gamma - 2\beta))}{(4\beta^2 - \gamma^2)^2}$$

$$\#66: \quad \frac{d}{d\lambda} \left( \text{eprofitxf} = \frac{\beta \cdot (2 \cdot T \cdot \beta \cdot \lambda + (c - \alpha) \cdot (2\beta - \gamma))^2}{(4\beta^2 - \gamma^2)^2} \right)$$

eq (C.1)

$$\#67: \quad \frac{4 \cdot T \cdot \beta^2 \cdot (2 \cdot T \cdot \beta \cdot \lambda + (c - \alpha) \cdot (2\beta - \gamma))}{(4\beta^2 - \gamma^2)^2}$$

&lt; 0 if [Assumption 3]

$$\#68: \quad 4 \cdot T \cdot \beta^2 \cdot (2 \cdot T \cdot \beta \cdot \lambda + (c - \alpha) \cdot (2\beta - \gamma)) < 0$$

$$\#69: \text{SOLVE}(4 \cdot T \cdot \beta^2 \cdot (2 \cdot T \cdot \beta \cdot \lambda + (c - \alpha) \cdot (2 \cdot \beta - \gamma)) < 0, T)$$

$$\begin{aligned} \#70: & \left( \beta \neq 0 \wedge T < 0 \wedge \text{IF} \left( \beta \cdot \lambda < 0, T < \frac{(c - \alpha) \cdot (\gamma - 2 \cdot \beta)}{2 \cdot \beta \cdot \lambda} \right) \right) \vee \left( \beta \neq 0 \wedge T < 0 \wedge \text{IF} \left( \beta \cdot \lambda > 0, T > \right. \right. \\ & \left. \left. \frac{(c - \alpha) \cdot (\gamma - 2 \cdot \beta)}{2 \cdot \beta \cdot \lambda} \right) \right) \vee \left( \beta \neq 0 \wedge T > 0 \wedge \text{IF} \left( \beta \cdot \lambda < 0, T > \frac{(c - \alpha) \cdot (\gamma - 2 \cdot \beta)}{2 \cdot \beta \cdot \lambda} \right) \right) \vee \left( \beta \neq 0 \wedge T > 0 \right. \\ & \left. \wedge \text{IF} \left( \beta \cdot \lambda > 0, T < \frac{(c - \alpha) \cdot (\gamma - 2 \cdot \beta)}{2 \cdot \beta \cdot \lambda} \right) \right) \end{aligned}$$

eq (C.2)

$$\#71: T < \frac{(c - \alpha) \cdot (\gamma - 2 \cdot \beta)}{2 \cdot \beta \cdot \lambda}$$

\*\*\* Section 4: Ad-valorem tariff wars

eq (10) profit X

$$\#72: \text{eprofitxh} = (pxh - c) \cdot xh$$

$$\#73: \text{eprofitxf} = \lambda \cdot ((1 - \tau) \cdot pxf - c) \cdot xf + (1 - \lambda) \cdot (pxf - c) \cdot xf$$

$$\#74: \text{eprofitx} = (pxh - c) \cdot xh + \lambda \cdot ((1 - \tau) \cdot pxf - c) \cdot xf + (1 - \lambda) \cdot (pxf - c) \cdot xf$$

eq (11) profit Y

$$\#75: \text{eprofityf} = (pyf - c) \cdot yf$$

$$\#76: \text{eprofityh} = \lambda \cdot ((1 - \tau) \cdot pyh - c) \cdot yh + (1 - \lambda) \cdot (pyh - c) \cdot yh$$

$$\#77: \text{eprofity} = (pyf - c) \cdot yf + \lambda \cdot ((1 - \tau) \cdot pyh - c) \cdot yh + (1 - \lambda) \cdot (pyh - c) \cdot yh$$

Derivations of (12) and (13) equilibrium sales and Appendix E

$$\#78: \text{eprofit}_x = ((\alpha - \beta \cdot x_h - \gamma \cdot y_h) - c) \cdot x_h + \lambda \cdot ((1 - \tau) \cdot (\alpha - \beta \cdot x_f - \gamma \cdot y_f) - c) \cdot x_f + (1 - \lambda) \cdot ((\alpha - \beta \cdot x_f - \gamma \cdot y_f) - c) \cdot x_f$$

$$\#79: \text{eprofit}_y = ((\alpha - \gamma \cdot x_f - \beta \cdot y_f) - c) \cdot y_f + \lambda \cdot ((1 - \tau) \cdot (\alpha - \gamma \cdot x_h - \beta \cdot y_h) - c) \cdot y_h + (1 - \lambda) \cdot ((\alpha - \gamma \cdot x_h - \beta \cdot y_h) - c) \cdot y_h$$

eqs (D.1)

$$\#80: \frac{d}{d x_f} (\text{eprofit}_x = ((\alpha - \beta \cdot x_h - \gamma \cdot y_h) - c) \cdot x_h + \lambda \cdot ((1 - \tau) \cdot (\alpha - \beta \cdot x_f - \gamma \cdot y_f) - c) \cdot x_f + (1 - \lambda) \cdot ((\alpha - \beta \cdot x_f - \gamma \cdot y_f) - c) \cdot x_f)$$

$$\#81: 0 = (2 \cdot x_f \cdot \beta + y_f \cdot \gamma - \alpha) \cdot (\lambda \cdot \tau - 1) - c$$

$$\#82: \frac{d}{d x_h} (\text{eprofit}_x = ((\alpha - \beta \cdot x_h - \gamma \cdot y_h) - c) \cdot x_h + \lambda \cdot ((1 - \tau) \cdot (\alpha - \beta \cdot x_f - \gamma \cdot y_f) - c) \cdot x_f + (1 - \lambda) \cdot ((\alpha - \beta \cdot x_f - \gamma \cdot y_f) - c) \cdot x_f)$$

$$\#83: 0 = -c - 2 \cdot x_h \cdot \beta - y_h \cdot \gamma + \alpha$$

eqs (D.2)

$$\#84: \frac{d}{d y_f} (\text{eprofit}_y = ((\alpha - \gamma \cdot x_f - \beta \cdot y_f) - c) \cdot y_f + \lambda \cdot ((1 - \tau) \cdot (\alpha - \gamma \cdot x_h - \beta \cdot y_h) - c) \cdot y_h + (1 - \lambda) \cdot ((\alpha - \gamma \cdot x_h - \beta \cdot y_h) - c) \cdot y_h)$$

$$\gamma \cdot xh - \beta \cdot yh) - c) \cdot yh)$$

$$\#85: \quad 0 = -c - xf \cdot \gamma - 2 \cdot yf \cdot \beta + \alpha$$

$$\#86: \quad \frac{d}{d \, yh} (\text{eprofit} = ((\alpha - \gamma \cdot xf - \beta \cdot yf) - c) \cdot yf + \lambda \cdot ((1 - \tau) \cdot (\alpha - \gamma \cdot xh - \beta \cdot yh) - c) \cdot yh + (1 - \lambda) \cdot ((\alpha -$$

$$\gamma \cdot xh - \beta \cdot yh) - c) \cdot yh)$$

$$\#87: \quad 0 = (xh \cdot \gamma + 2 \cdot yh \cdot \beta - \alpha) \cdot (\lambda \cdot \tau - 1) - c$$

$$\#88: \quad \text{SOLVE}([0 = (2 \cdot xf \cdot \beta + yf \cdot \gamma - \alpha) \cdot (\lambda \cdot \tau - 1) - c, 0 = -c - 2 \cdot xh \cdot \beta - yh \cdot \gamma + \alpha, 0 = -c - xf \cdot \gamma - 2 \cdot yf \cdot \beta + \alpha, 0 = (xh \cdot \gamma + 2 \cdot yh \cdot \beta - \alpha) \cdot (\lambda \cdot \tau - 1) - c], [xf, xh, yf, yh])$$

eqs (13) and (14)

$$\#89: \quad \left[ \begin{aligned} xf &= \frac{c \cdot (2 \cdot \beta + \gamma \cdot (\lambda \cdot \tau - 1)) + \alpha \cdot (2 \cdot \beta - \gamma) \cdot (\lambda \cdot \tau - 1)}{(4 \cdot \beta^2 - \gamma^2) \cdot (\lambda \cdot \tau - 1)} \wedge xh = \\ &\frac{c \cdot (2 \cdot \beta \cdot (\lambda \cdot \tau - 1) + \gamma) + \alpha \cdot (1 - \lambda \cdot \tau) \cdot (2 \cdot \beta - \gamma)}{(1 - \lambda \cdot \tau) \cdot (4 \cdot \beta^2 - \gamma^2)} \wedge yf = \\ &\frac{c \cdot (2 \cdot \beta \cdot (\lambda \cdot \tau - 1) + \gamma) + \alpha \cdot (1 - \lambda \cdot \tau) \cdot (2 \cdot \beta - \gamma)}{(1 - \lambda \cdot \tau) \cdot (4 \cdot \beta^2 - \gamma^2)} \wedge yh = \end{aligned} \right.$$

$$\left. \frac{c \cdot (2 \cdot \beta + \gamma \cdot (\lambda \cdot \tau - 1)) + \alpha \cdot (2 \cdot \beta - \gamma) \cdot (\lambda \cdot \tau - 1)}{(4 \cdot \beta^2 - \gamma^2) \cdot (\lambda \cdot \tau - 1)} \right]$$

xh = yf > 0 if

$$\#90: \quad c \cdot (2 \cdot \beta \cdot (\lambda \cdot \tau - 1) + \gamma) + \alpha \cdot (1 - \lambda \cdot \tau) \cdot (2 \cdot \beta - \gamma) > 0$$

$$\#91: \quad \text{SOLVE}(c \cdot (2 \cdot \beta \cdot (\lambda \cdot \tau - 1) + \gamma) + \alpha \cdot (1 - \lambda \cdot \tau) \cdot (2 \cdot \beta - \gamma) > 0, \tau)$$

$$\#92: \quad \text{IF} \left( 2 \cdot c \cdot \beta \cdot \lambda + \alpha \cdot \lambda \cdot (\gamma - 2 \cdot \beta) < 0, \tau < \frac{(c - \alpha) \cdot (2 \cdot \beta - \gamma)}{\lambda \cdot (2 \cdot c \cdot \beta + \alpha \cdot (\gamma - 2 \cdot \beta))} \right) \vee \text{IF} \left( 2 \cdot c \cdot \beta \cdot \lambda + \alpha \cdot \lambda \cdot (\gamma - 2 \cdot \beta) > 0, \tau > \frac{(c - \alpha) \cdot (2 \cdot \beta - \gamma)}{\lambda \cdot (2 \cdot c \cdot \beta + \alpha \cdot (\gamma - 2 \cdot \beta))} \right)$$

Assumption 4 (first term)

$$\#93: \quad \tau < \frac{(c - \alpha) \cdot (2 \cdot \beta - \gamma)}{\lambda \cdot (2 \cdot c \cdot \beta + \alpha \cdot (\gamma - 2 \cdot \beta))}$$

xf = yh > 0 if

$$\#94: \quad c \cdot (2 \cdot \beta + \gamma \cdot (\lambda \cdot \tau - 1)) + \alpha \cdot (2 \cdot \beta - \gamma) \cdot (\lambda \cdot \tau - 1) < 0$$

$$\#95: \quad \text{SOLVE}(c \cdot (2 \cdot \beta + \gamma \cdot (\lambda \cdot \tau - 1)) + \alpha \cdot (2 \cdot \beta - \gamma) \cdot (\lambda \cdot \tau - 1) < 0, \tau)$$

$$\#96: \quad \text{IF} \left( c \cdot \gamma \cdot \lambda + \alpha \cdot \lambda \cdot (2 \cdot \beta - \gamma) < 0, \tau > \frac{(c - \alpha) \cdot (\gamma - 2 \cdot \beta)}{\lambda \cdot (c \cdot \gamma + \alpha \cdot (2 \cdot \beta - \gamma))} \right) \vee \text{IF} \left( c \cdot \gamma \cdot \lambda + \alpha \cdot \lambda \cdot (2 \cdot \beta - \gamma) > 0, \tau < \frac{(c - \alpha) \cdot (\gamma - 2 \cdot \beta)}{\lambda \cdot (c \cdot \gamma + \alpha \cdot (2 \cdot \beta - \gamma))} \right)$$

Assumption 4 (second term)

$$\#97: \tau < \frac{(c - \alpha) \cdot (\gamma - 2 \cdot \beta)}{\lambda \cdot (c \cdot \gamma + \alpha \cdot (2 \cdot \beta - \gamma))}$$

which one is higher?

$$\#98: \frac{(c - \alpha) \cdot (2 \cdot \beta - \gamma)}{\lambda \cdot (2 \cdot c \cdot \beta + \alpha \cdot (\gamma - 2 \cdot \beta))} - \frac{(c - \alpha) \cdot (\gamma - 2 \cdot \beta)}{\lambda \cdot (c \cdot \gamma + \alpha \cdot (2 \cdot \beta - \gamma))}$$

$$\#99: \frac{c \cdot (c - \alpha) \cdot (2 \cdot \beta + \gamma) \cdot (2 \cdot \beta - \gamma)}{\lambda \cdot (2 \cdot c \cdot \beta + \alpha \cdot (\gamma - 2 \cdot \beta)) \cdot (c \cdot \gamma + \alpha \cdot (2 \cdot \beta - \gamma))}$$

$$\#100: p_{xh} = \frac{c \cdot (2 \cdot \beta^2 \cdot (\lambda \cdot \tau - 1) - \beta \cdot \gamma + \gamma^2 \cdot (1 - \lambda \cdot \tau)) + \alpha \cdot \beta \cdot (2 \cdot \beta - \gamma) \cdot (\lambda \cdot \tau - 1)}{(4 \cdot \beta^2 - \gamma^2) \cdot (\lambda \cdot \tau - 1)}$$

$$\#101: p_{yh} = \frac{c \cdot (2 \cdot \beta^2 + \beta \cdot \gamma \cdot (1 - \lambda \cdot \tau) - \gamma^2) + \alpha \cdot \beta \cdot (1 - \lambda \cdot \tau) \cdot (2 \cdot \beta - \gamma)}{(1 - \lambda \cdot \tau) \cdot (4 \cdot \beta^2 - \gamma^2)}$$

$$\#102: p_{xf} = \frac{c \cdot (2 \cdot \beta^2 + \beta \cdot \gamma \cdot (1 - \lambda \cdot \tau) - \gamma^2) + \alpha \cdot \beta \cdot (1 - \lambda \cdot \tau) \cdot (2 \cdot \beta - \gamma)}{(1 - \lambda \cdot \tau) \cdot (4 \cdot \beta^2 - \gamma^2)}$$

$$\#103: p_{yf} = \frac{c \cdot (2 \cdot \beta^2 \cdot (\lambda \cdot \tau - 1) - \beta \cdot \gamma + \gamma^2 \cdot (1 - \lambda \cdot \tau)) + \alpha \cdot \beta \cdot (2 \cdot \beta - \gamma) \cdot (\lambda \cdot \tau - 1)}{(4 \cdot \beta^2 - \gamma^2) \cdot (\lambda \cdot \tau - 1)}$$

eqs (14): equilibrium expected domestic profits

$$\#104: \quad eprofitxh = \frac{\beta \cdot (c \cdot (2 \cdot \beta \cdot (\lambda \cdot \tau - 1) + \gamma) + \alpha \cdot (1 - \lambda \cdot \tau) \cdot (2 \cdot \beta - \gamma))^2}{(4 \cdot \beta^2 - \gamma^2) \cdot (\lambda \cdot \tau - 1)^2}$$

$$\#105: \quad eprofityf = \frac{\beta \cdot (c \cdot (2 \cdot \beta \cdot (\lambda \cdot \tau - 1) + \gamma) + \alpha \cdot (1 - \lambda \cdot \tau) \cdot (2 \cdot \beta - \gamma))^2}{(4 \cdot \beta^2 - \gamma^2) \cdot (\lambda \cdot \tau - 1)^2}$$

eqs (15): equilibrium expected export profits

$$\#106: \quad eprofitxf = \frac{\beta \cdot (c \cdot (2 \cdot \beta + \gamma \cdot (\lambda \cdot \tau - 1)) + \alpha \cdot (2 \cdot \beta - \gamma) \cdot (\lambda \cdot \tau - 1))^2}{(1 - \lambda \cdot \tau) \cdot (4 \cdot \beta^2 - \gamma^2)}$$

$$\#107: \quad eprofityh = \frac{\beta \cdot (c \cdot (2 \cdot \beta + \gamma \cdot (\lambda \cdot \tau - 1)) + \alpha \cdot (2 \cdot \beta - \gamma) \cdot (\lambda \cdot \tau - 1))^2}{(1 - \lambda \cdot \tau) \cdot (4 \cdot \beta^2 - \gamma^2)}$$

\*\*\* Section 5: Unilateral tariff with no retaliation

eq (16) profit of X

$$\#108: \quad eprofitx = (pxh - c) \cdot xh + (pxf - c) \cdot xf$$

eq (17) profit of Y

$$\#109: \quad eprofity = (pyf - c) \cdot yf + \lambda \cdot (pyh - c - T) \cdot yh + (1 - \lambda) \cdot (pyh - c) \cdot yh$$

Appendix E

$$\#110: \text{eprofitx} = ((\alpha - \beta \cdot x_h - \gamma \cdot y_h) - c) \cdot x_h + ((\alpha - \beta \cdot x_f - \gamma \cdot y_f) - c) \cdot x_f$$

$$\#111: \text{eprofity} = ((\alpha - \gamma \cdot x_f - \beta \cdot y_f) - c) \cdot y_f + \lambda \cdot ((\alpha - \gamma \cdot x_h - \beta \cdot y_h) - c - T) \cdot y_h + (1 - \lambda) \cdot ((\alpha - \gamma \cdot x_h - \beta \cdot y_h) - c) \cdot y_h$$

eqs (E.1)

$$\#112: \frac{d}{d x_f} (\text{eprofitx} = ((\alpha - \beta \cdot x_h - \gamma \cdot y_h) - c) \cdot x_h + ((\alpha - \beta \cdot x_f - \gamma \cdot y_f) - c) \cdot x_f)$$

$$\#113: 0 = -c - 2 \cdot x_f \cdot \beta - y_f \cdot \gamma + \alpha$$

$$\#114: \frac{d}{d x_h} (\text{eprofitx} = ((\alpha - \beta \cdot x_h - \gamma \cdot y_h) - c) \cdot x_h + ((\alpha - \beta \cdot x_f - \gamma \cdot y_f) - c) \cdot x_f)$$

$$\#115: 0 = -c - 2 \cdot x_h \cdot \beta - y_h \cdot \gamma + \alpha$$

eqs (E.2)

$$\#116: \frac{d}{d y_f} (\text{eprofity} = ((\alpha - \gamma \cdot x_f - \beta \cdot y_f) - c) \cdot y_f + \lambda \cdot ((\alpha - \gamma \cdot x_h - \beta \cdot y_h) - c - T) \cdot y_h + (1 - \lambda) \cdot ((\alpha - \gamma \cdot x_h - \beta \cdot y_h) - c) \cdot y_h)$$

$$\#117: 0 = -c - x_f \cdot \gamma - 2 \cdot y_f \cdot \beta + \alpha$$

$$\#118: \frac{d}{d y_h} (\text{eprofity} = ((\alpha - \gamma \cdot x_f - \beta \cdot y_f) - c) \cdot y_f + \lambda \cdot ((\alpha - \gamma \cdot x_h - \beta \cdot y_h) - c - T) \cdot y_h + (1 - \lambda) \cdot ((\alpha - \gamma \cdot x_h - \beta \cdot y_h) - c) \cdot y_h)$$



$$\gamma \cdot x_h - \beta \cdot y_h) - c) \cdot y_h)$$

$$\#119: \quad 0 = -T \cdot \lambda - c - x_h \cdot \gamma - 2 \cdot y_h \cdot \beta + \alpha$$

eq (18) eq1 sales under no retaliation

$$\#120: \text{SOLVE}([0 = -c - 2 \cdot x_f \cdot \beta - y_f \cdot \gamma + \alpha, 0 = -c - 2 \cdot x_h \cdot \beta - y_h \cdot \gamma + \alpha, 0 = -c - x_f \cdot \gamma - 2 \cdot y_f \cdot \beta + \alpha, 0 = -T \cdot \lambda - c - x_h \cdot \gamma - 2 \cdot y_h \cdot \beta + \alpha], [x_f, x_h, y_f, y_h])$$

$$\#121: \left[ x_f = \frac{\alpha - c}{2 \cdot \beta + \gamma} \wedge x_h = \frac{T \cdot \gamma \cdot \lambda + (c - \alpha) \cdot (\gamma - 2 \cdot \beta)}{4 \cdot \beta^2 - \gamma^2} \wedge y_f = \frac{\alpha - c}{2 \cdot \beta + \gamma} \wedge y_h = \frac{2 \cdot T \cdot \beta \cdot \lambda + (c - \alpha) \cdot (2 \cdot \beta - \gamma)}{\gamma^2 - 4 \cdot \beta^2} \right]$$

$y > 0$  if [Assumption 3]

$$\#122: 2 \cdot T \cdot \beta \cdot \lambda + (c - \alpha) \cdot (2 \cdot \beta - \gamma) < 0$$

$$\#123: \text{SOLVE}(2 \cdot T \cdot \beta \cdot \lambda + (c - \alpha) \cdot (2 \cdot \beta - \gamma) < 0, T)$$

$$\#124: \quad \text{IF} \left( \beta \cdot \lambda < 0, T > \frac{(c - \alpha) \cdot (\gamma - 2 \cdot \beta)}{2 \cdot \beta \cdot \lambda} \right) \vee \text{IF} \left( \beta \cdot \lambda > 0, T < \frac{(c - \alpha) \cdot (\gamma - 2 \cdot \beta)}{2 \cdot \beta \cdot \lambda} \right)$$

$$\#125: T < \frac{(c - \alpha) \cdot (\gamma - 2 \cdot \beta)}{2 \cdot \beta \cdot \lambda}$$

eq (E.3) equilibrium prices without retaliation

$$\#126: \quad p_{xh} = \frac{T \cdot \beta \cdot \gamma \cdot \lambda + (2 \cdot \beta - \gamma) \cdot (c \cdot (\beta + \gamma) + \alpha \cdot \beta)}{4 \cdot \beta^2 - \gamma^2}$$

$$\#127: \quad p_{yh} = \frac{T \cdot \lambda \cdot (2 \cdot \beta^2 - \gamma^2) + (2 \cdot \beta - \gamma) \cdot (c \cdot (\beta + \gamma) + \alpha \cdot \beta)}{4 \cdot \beta^2 - \gamma^2}$$

$$\#128: \quad p_{xf} = \frac{c \cdot (\beta + \gamma) + \alpha \cdot \beta}{2 \cdot \beta + \gamma}$$

$$\#129: \quad p_{yf} = \frac{c \cdot (\beta + \gamma) + \alpha \cdot \beta}{2 \cdot \beta + \gamma}$$

eq (19) equilibrium profit of X without retaliation

$$\#130: \quad eprofit_x = \frac{\beta \cdot (T \cdot \gamma \cdot \lambda^2 + 2 \cdot T \cdot \gamma \cdot \lambda \cdot (c - \alpha) \cdot (\gamma - 2 \cdot \beta) + 2 \cdot (c - \alpha)^2 \cdot (2 \cdot \beta - \gamma)^2)}{(2 \cdot \beta + \gamma)^2 \cdot (2 \cdot \beta - \gamma)^2}$$

eq (20) equilibrium profit of Y without retaliation

$$\#131: \quad eprofit_y = \frac{2 \cdot \beta \cdot (2 \cdot T \cdot \beta^2 \cdot \lambda^2 + 2 \cdot T \cdot \beta \cdot \lambda \cdot (c - \alpha) \cdot (2 \cdot \beta - \gamma) + (c - \alpha)^2 \cdot (2 \cdot \beta - \gamma)^2)}{(2 \cdot \beta + \gamma)^2 \cdot (2 \cdot \beta - \gamma)^2}$$

Result 4 and Appendix F

eq (F.1)

$$\#132: \frac{d}{d\lambda} \left( \text{eprofit}_x = \frac{\beta \cdot (T \cdot \gamma \cdot \lambda^2 + 2 \cdot T \cdot \gamma \cdot \lambda \cdot (c - \alpha) \cdot (\gamma - 2 \cdot \beta) + 2 \cdot (c - \alpha)^2 \cdot (2 \cdot \beta - \gamma)^2)}{(2 \cdot \beta + \gamma)^2 \cdot (2 \cdot \beta - \gamma)^2} \right)$$

$$\#133: 0 > \frac{2 \cdot T \cdot \beta \cdot \gamma \cdot (T \cdot \gamma \cdot \lambda + (c - \alpha) \cdot (\gamma - 2 \cdot \beta))}{(2 \cdot \beta + \gamma)^2 \cdot (2 \cdot \beta - \gamma)^2}$$

eq (F.2)

$$\#134: \frac{d}{d\lambda} \left( \text{eprofit}_y = \frac{2 \cdot \beta \cdot (2 \cdot T \cdot \beta \cdot \lambda^2 + 2 \cdot T \cdot \beta \cdot \lambda \cdot (c - \alpha) \cdot (2 \cdot \beta - \gamma) + (c - \alpha)^2 \cdot (2 \cdot \beta - \gamma)^2)}{(2 \cdot \beta + \gamma)^2 \cdot (2 \cdot \beta - \gamma)^2} \right)$$

$$\#135: \frac{4 \cdot T \cdot \beta^2 \cdot (2 \cdot T \cdot \beta \cdot \lambda + (c - \alpha) \cdot (2 \cdot \beta - \gamma))}{(2 \cdot \beta + \gamma)^2 \cdot (2 \cdot \beta - \gamma)^2}$$

&lt; 0 if [Assumption 3]

$$\#136: 2 \cdot T \cdot \beta \cdot \lambda + (c - \alpha) \cdot (2 \cdot \beta - \gamma) < 0$$

$$\#137: \text{SOLVE}(2 \cdot T \cdot \beta \cdot \lambda + (c - \alpha) \cdot (2 \cdot \beta - \gamma) < 0, T)$$

$$\#138: \text{IF} \left( \beta \cdot \lambda < 0, T > \frac{(c - \alpha) \cdot (\gamma - 2 \cdot \beta)}{2 \cdot \beta \cdot \lambda} \right) \vee \text{IF} \left( \beta \cdot \lambda > 0, T < \frac{(c - \alpha) \cdot (\gamma - 2 \cdot \beta)}{2 \cdot \beta \cdot \lambda} \right)$$

$$\#139: T < \frac{(c - \alpha) \cdot (\gamma - 2 \cdot \beta)}{2 \cdot \beta \cdot \lambda}$$